theories/laws/utp_alpha_laws.thy
@@ -1,0 +1,34 @@
+(******************************************************************************)
+(* Project: Unifying Theories of Programming in HOL                           *)
+(* File: utp_alpha_laws.thy                                                   *)
+(* Author: Simon Foster and Frank Zeyda, University of York (UK)              *)
+(******************************************************************************)
+
+header {* Alphabetised Predicate and Relation Laws *}
+
+theory utp_alpha_laws
+imports 
+  "../alpha/utp_alpha_pred"
+  "../alpha/utp_alpha_expr"
+  "../alpha/utp_alpha_rel"
+  "../tactics/utp_alpha_tac"
+  "../tactics/utp_alpha_expr_tac"
+  utp_pred_laws
+  utp_rename_laws
+  utp_subst_laws
+  utp_rel_laws
+begin
+
+theorem SemiA_extract_variable:
+  assumes 
+    "x \<in> D\<^sub>0" "x\<acute> \<in>\<^sub>f \<alpha> P" "x \<in>\<^sub>f \<alpha> Q"
+    "x\<acute>\<acute> \<notin>\<^sub>f \<alpha> P" "x\<acute>\<acute> \<notin>\<^sub>f \<alpha> Q"
+  shows "P ;\<^sub>\<alpha> Q = (\<exists>-\<^sub>\<alpha> \<lbrace>x\<acute>\<acute>\<rbrace>. P[$\<^sub>\<alpha>x\<acute>\<acute>/\<^sub>\<alpha>x\<acute>] ;\<^sub>\<alpha> Q[$\<^sub>\<alpha>x\<acute>\<acute>/\<^sub>\<alpha>x])"
+  using assms
+  apply (utp_alpha_tac)
+  apply (auto)[1]
+  apply (rule SemiR_extract_variable)
+  apply (simp_all add:unrest)
+done
+
+end
